code/experimental/P256/Hacl.Test.fst
@@ -1,0 +1,19 @@
+module Hacl.Test
+
+open Lib.IntTypes
+open FStar.Math.Lemmas
+open FStar.Mul
+
+open Lib.Sequence
+open Lib.ByteSequence
+
+friend Lib.ByteSequence 
+
+#set-options "--z3rlimit 100"
+
+val lemma_core1: k: lseq uint64 4 -> Lemma
+    (nat_from_bytes_le (uints_to_bytes_le k) == nat_from_intseq_le k)
+
+
+let lemma_core1 k = 
+  lemma_nat
